Working on ntt.poly_element_sample_cbd_from_bytes_eta2_inner_loop.spec but encountering significant slowdown

proofs/Symcrust/Properties/SamplePolyCBD/SamplePolyCBD.lean
@@ -27,7 +27,207 @@ namespace Symcrust.SpecAux
 open Symcrust.Spec Symcrust.ntt
 open Aeneas Aeneas.Std Aeneas.SRRange Result
 
-set_option maxHeartbeats 1000000
+set_option maxHeartbeats 2000000
+
+theorem ntt.poly_element_sample_cbd_from_bytes_eta2_inner_loop.spec.aux
+  (f : Std.Array U16 256#usize) (i : Usize) (sample_bits : U32) (hi1 : i.val < 256) (hi2 : 8 ∣ i.val)
+  (coefficient_1 : U32)
+  (coefficient_post_1_1 : ↑coefficient_1 = ↑(sample_bits &&& 15#u32))
+  (sample_bits1_1 : U32)
+  (sample_bits1_post_1_1 : ↑sample_bits1_1 = ↑sample_bits >>> 4)
+  (sample_bits1_post_2_1 : sample_bits1_1.bv = sample_bits.bv >>> 4) (i1_1 : U32)
+  (i1_post_1_1 : ↑i1_1 = ↑(coefficient_1 &&& 3#u32))
+  (i2_1 : U32) (i2_post_1_1 : ↑i2_1 = ↑coefficient_1 >>> 2) (i2_post_2_1 : i2_1.bv = coefficient_1.bv >>> 2)
+  (coefficient1_1 : U32) (coefficient1_post_1 : coefficient1_1 = core.num.U32.wrapping_sub i1_1 i2_1) (i3_1 : U32)
+  (i3_post_1_1 : ↑i3_1 = ↑coefficient1_1 >>> 16) (i3_post_2_1 : i3_1.bv = coefficient1_1.bv >>> 16) (i4_1 : U32)
+  (i4_post_1_1 : ↑i4_1 = ↑(3329#u32 &&& i3_1)) (coefficient2_1 : U32)
+  (coefficient2_post_1 : coefficient2_1 = core.num.U32.wrapping_add coefficient1_1 i4_1) (i5_1 : Usize)
+  (i5_post_1 : ↑i5_1 = i.val + 0) (i6_1 : U16) (i6_post_1 : i6_1 = UScalar.cast UScalarTy.U16 coefficient2_1)
+  (pe_dst1_1 : Std.Array U16 256#usize) (pe_dst1_post_1 : pe_dst1_1 = f.set i5_1 i6_1) (j1_1 : Usize)
+  (j1_post_1 : j1_1.val = 1) (coefficient_2 : U32)
+  (coefficient_post_1_2 : ↑coefficient_2 = ↑(sample_bits1_1 &&& 15#u32)) (sample_bits1_2 : U32)
+  (sample_bits1_post_1_2 : ↑sample_bits1_2 = ↑sample_bits1_1 >>> 4)
+  (sample_bits1_post_2_2 : sample_bits1_2.bv = sample_bits1_1.bv >>> 4) (i1_2 : U32)
+  (i1_post_1_2 : ↑i1_2 = ↑(coefficient_2 &&& 3#u32))
+  (i2_2 : U32) (i2_post_1_2 : ↑i2_2 = ↑coefficient_2 >>> 2) (i2_post_2_2 : i2_2.bv = coefficient_2.bv >>> 2)
+  (coefficient1_2 : U32) (coefficient1_post_2 : coefficient1_2 = core.num.U32.wrapping_sub i1_2 i2_2) (i3_2 : U32)
+  (i3_post_1_2 : ↑i3_2 = ↑coefficient1_2 >>> 16) (i3_post_2_2 : i3_2.bv = coefficient1_2.bv >>> 16) (i4_2 : U32)
+  (i4_post_1_2 : ↑i4_2 = ↑(3329#u32 &&& i3_2)) (coefficient2_2 : U32)
+  (coefficient2_post_2 : coefficient2_2 = core.num.U32.wrapping_add coefficient1_2 i4_2) (i5_2 : Usize)
+  (i5_post_2 : ↑i5_2 = ↑i + j1_1.val) (i6_2 : U16) (i6_post_2 : i6_2 = UScalar.cast UScalarTy.U16 coefficient2_2)
+  (pe_dst1_2 : Std.Array U16 256#usize) (pe_dst1_post_2 : pe_dst1_2 = pe_dst1_1.set i5_2 i6_2) (j1_2 : Usize)
+  (j1_post_2 : ↑j1_2 = j1_1.val + 1) (h : j1_2 < 8#usize) (coefficient_3 : U32)
+  (coefficient_post_1_3 : ↑coefficient_3 = ↑(sample_bits1_2 &&& 15#u32))
+  (sample_bits1_3 : U32)
+  (sample_bits1_post_1_3 : ↑sample_bits1_3 = ↑sample_bits1_2 >>> 4)
+  (sample_bits1_post_2_3 : sample_bits1_3.bv = sample_bits1_2.bv >>> 4) (i1_3 : U32)
+  (i1_post_1_3 : ↑i1_3 = ↑(coefficient_3 &&& 3#u32))
+  (i2_3 : U32) (i2_post_1_3 : ↑i2_3 = ↑coefficient_3 >>> 2) (i2_post_2_3 : i2_3.bv = coefficient_3.bv >>> 2)
+  (coefficient1_3 : U32) (coefficient1_post_3 : coefficient1_3 = core.num.U32.wrapping_sub i1_3 i2_3) (i3_3 : U32)
+  (i3_post_1_3 : ↑i3_3 = ↑coefficient1_3 >>> 16) (i3_post_2_3 : i3_3.bv = coefficient1_3.bv >>> 16) (i4_3 : U32)
+  (i4_post_1_3 : ↑i4_3 = ↑(ntt.Q &&& i3_3)) (i4_post_2_3 : i4_3.bv = ntt.Q.bv &&& i3_3.bv) (coefficient2_3 : U32)
+  (coefficient2_post_3 : coefficient2_3 = core.num.U32.wrapping_add coefficient1_3 i4_3) (i5_3 : Usize)
+  (i5_post_3 : ↑i5_3 = i.val + ↑j1_2) (i6_3 : U16) (i6_post_3 : i6_3 = UScalar.cast UScalarTy.U16 coefficient2_3)
+  (pe_dst1_3 : Std.Array U16 256#usize) (pe_dst1_post_3 : pe_dst1_3 = pe_dst1_2.set i5_3 i6_3) (j1_3 : Usize)
+  (j1_post_3 : ↑j1_3 = j1_2.val + 1) (h_1 : j1_3 < 8#usize) (coefficient_4 : U32)
+  (coefficient_post_1_4 : ↑coefficient_4 = ↑(sample_bits1_3 &&& 15#u32))
+  (sample_bits1_4 : U32)
+  (sample_bits1_post_1_4 : ↑sample_bits1_4 = ↑sample_bits1_3 >>> 4)
+  (sample_bits1_post_2_4 : sample_bits1_4.bv = sample_bits1_3.bv >>> 4) (i1_4 : U32)
+  (i1_post_1_4 : ↑i1_4 = ↑(coefficient_4 &&& 3#u32))
+  (i2_4 : U32) (i2_post_1_4 : ↑i2_4 = ↑coefficient_4 >>> 2) (i2_post_2_4 : i2_4.bv = coefficient_4.bv >>> 2)
+  (coefficient1_4 : U32) (coefficient1_post_4 : coefficient1_4 = core.num.U32.wrapping_sub i1_4 i2_4) (i3_4 : U32)
+  (i3_post_1_4 : ↑i3_4 = ↑coefficient1_4 >>> 16) (i3_post_2_4 : i3_4.bv = coefficient1_4.bv >>> 16) (i4_4 : U32)
+  (i4_post_1_4 : ↑i4_4 = ↑(ntt.Q &&& i3_4)) (i4_post_2_4 : i4_4.bv = ntt.Q.bv &&& i3_4.bv) (coefficient2_4 : U32)
+  (coefficient2_post_4 : coefficient2_4 = core.num.U32.wrapping_add coefficient1_4 i4_4) (i5_4 : Usize)
+  (i5_post_4 : ↑i5_4 = i.val + ↑j1_3) (i6_4 : U16) (i6_post_4 : i6_4 = UScalar.cast UScalarTy.U16 coefficient2_4)
+  (pe_dst1_4 : Std.Array U16 256#usize) (pe_dst1_post_4 : pe_dst1_4 = pe_dst1_3.set i5_4 i6_4) (j1_4 : Usize)
+  (j1_post_4 : ↑j1_4 = j1_3.val + 1) (h_2 : j1_4 < 8#usize) (coefficient_5 : U32)
+  (coefficient_post_1_5 : ↑coefficient_5 = ↑(sample_bits1_4 &&& 15#u32))
+  (sample_bits1_5 : U32)
+  (sample_bits1_post_1_5 : ↑sample_bits1_5 = ↑sample_bits1_4 >>> 4)
+  (sample_bits1_post_2_5 : sample_bits1_5.bv = sample_bits1_4.bv >>> 4) (i1_5 : U32)
+  (i1_post_1_5 : ↑i1_5 = ↑(coefficient_5 &&& 3#u32))
+  (i2_5 : U32) (i2_post_1_5 : ↑i2_5 = ↑coefficient_5 >>> 2) (i2_post_2_5 : i2_5.bv = coefficient_5.bv >>> 2)
+  (coefficient1_5 : U32) (coefficient1_post_5 : coefficient1_5 = core.num.U32.wrapping_sub i1_5 i2_5) (i3_5 : U32)
+  (i3_post_1_5 : ↑i3_5 = ↑coefficient1_5 >>> 16) (i3_post_2_5 : i3_5.bv = coefficient1_5.bv >>> 16) (i4_5 : U32)
+  (i4_post_1_5 : ↑i4_5 = ↑(ntt.Q &&& i3_5)) (i4_post_2_5 : i4_5.bv = ntt.Q.bv &&& i3_5.bv) (coefficient2_5 : U32)
+  (coefficient2_post_5 : coefficient2_5 = core.num.U32.wrapping_add coefficient1_5 i4_5) (i5_5 : Usize)
+  (i5_post_5 : ↑i5_5 = i.val + ↑j1_4) (i6_5 : U16) (i6_post_5 : i6_5 = UScalar.cast UScalarTy.U16 coefficient2_5)
+  (pe_dst1_5 : Std.Array U16 256#usize) (pe_dst1_post_5 : pe_dst1_5 = pe_dst1_4.set i5_5 i6_5) (j1_5 : Usize)
+  (j1_post_5 : ↑j1_5 = j1_4.val + 1) (h_3 : j1_5 < 8#usize) (coefficient_6 : U32)
+  (coefficient_post_1_6 : ↑coefficient_6 = ↑(sample_bits1_5 &&& 15#u32))
+  (sample_bits1_6 : U32)
+  (sample_bits1_post_1_6 : ↑sample_bits1_6 = ↑sample_bits1_5 >>> 4)
+  (sample_bits1_post_2_6 : sample_bits1_6.bv = sample_bits1_5.bv >>> 4) (i1_6 : U32)
+  (i1_post_1_6 : ↑i1_6 = ↑(coefficient_6 &&& 3#u32))
+  (i2_6 : U32) (i2_post_1_6 : ↑i2_6 = ↑coefficient_6 >>> 2) (i2_post_2_6 : i2_6.bv = coefficient_6.bv >>> 2)
+  (coefficient1_6 : U32) (coefficient1_post_6 : coefficient1_6 = core.num.U32.wrapping_sub i1_6 i2_6) (i3_6 : U32)
+  (i3_post_1_6 : ↑i3_6 = ↑coefficient1_6 >>> 16) (i3_post_2_6 : i3_6.bv = coefficient1_6.bv >>> 16) (i4_6 : U32)
+  (i4_post_1_6 : ↑i4_6 = ↑(ntt.Q &&& i3_6)) (i4_post_2_6 : i4_6.bv = ntt.Q.bv &&& i3_6.bv) (coefficient2_6 : U32)
+  (coefficient2_post_6 : coefficient2_6 = core.num.U32.wrapping_add coefficient1_6 i4_6) (i5_6 : Usize)
+  (i5_post_6 : ↑i5_6 = i.val + ↑j1_5) (i6_6 : U16) (i6_post_6 : i6_6 = UScalar.cast UScalarTy.U16 coefficient2_6)
+  (pe_dst1_6 : Std.Array U16 256#usize) (pe_dst1_post_6 : pe_dst1_6 = pe_dst1_5.set i5_6 i6_6) (j1_6 : Usize)
+  (j1_post_6 : ↑j1_6 = j1_5.val + 1) (h_4 : j1_6 < 8#usize) (coefficient_7 : U32)
+  (coefficient_post_1_7 : ↑coefficient_7 = ↑(sample_bits1_6 &&& 15#u32))
+  (sample_bits1_7 : U32)
+  (sample_bits1_post_1_7 : ↑sample_bits1_7 = ↑sample_bits1_6 >>> 4)
+  (sample_bits1_post_2_7 : sample_bits1_7.bv = sample_bits1_6.bv >>> 4) (i1_7 : U32)
+  (i1_post_1_7 : ↑i1_7 = ↑(coefficient_7 &&& 3#u32))
+  (i2_7 : U32) (i2_post_1_7 : ↑i2_7 = ↑coefficient_7 >>> 2) (i2_post_2_7 : i2_7.bv = coefficient_7.bv >>> 2)
+  (coefficient1_7 : U32) (coefficient1_post_7 : coefficient1_7 = core.num.U32.wrapping_sub i1_7 i2_7) (i3_7 : U32)
+  (i3_post_1_7 : ↑i3_7 = ↑coefficient1_7 >>> 16) (i3_post_2_7 : i3_7.bv = coefficient1_7.bv >>> 16) (i4_7 : U32)
+  (i4_post_1_7 : ↑i4_7 = ↑(ntt.Q &&& i3_7)) (i4_post_2_7 : i4_7.bv = ntt.Q.bv &&& i3_7.bv) (coefficient2_7 : U32)
+  (coefficient2_post_7 : coefficient2_7 = core.num.U32.wrapping_add coefficient1_7 i4_7) (i5_7 : Usize)
+  (i5_post_7 : ↑i5_7 = i.val + ↑j1_6) (i6_7 : U16) (i6_post_7 : i6_7 = UScalar.cast UScalarTy.U16 coefficient2_7)
+  (pe_dst1_7 : Std.Array U16 256#usize) (pe_dst1_post_7 : pe_dst1_7 = pe_dst1_6.set i5_7 i6_7) (j1_7 : Usize)
+  (j1_post_7 : ↑j1_7 = j1_6.val + 1) (h_5 : j1_7 < 8#usize) (coefficient : U32)
+  (coefficient_post_1 : ↑coefficient = ↑(sample_bits1_7 &&& 15#u32))
+  (sample_bits1 : U32)
+  (sample_bits1_post_1 : ↑sample_bits1 = ↑sample_bits1_7 >>> 4)
+  (sample_bits1_post_2 : sample_bits1.bv = sample_bits1_7.bv >>> 4) (i1 : U32)
+  (i1_post_1 : ↑i1 = ↑(coefficient &&& 3#u32)) (i2 : U32)
+  (i2_post_1 : ↑i2 = ↑coefficient >>> 2) (i2_post_2 : i2.bv = coefficient.bv >>> 2) (coefficient1 : U32)
+  (coefficient1_post : coefficient1 = core.num.U32.wrapping_sub i1 i2) (i3 : U32)
+  (i3_post_1 : ↑i3 = ↑coefficient1 >>> 16) (i3_post_2 : i3.bv = coefficient1.bv >>> 16) (i4 : U32)
+  (i4_post_1 : ↑i4 = ↑(ntt.Q &&& i3)) (i4_post_2 : i4.bv = ntt.Q.bv &&& i3.bv) (coefficient2 : U32)
+  (coefficient2_post : coefficient2 = core.num.U32.wrapping_add coefficient1 i4) (i5 : Usize)
+  (i5_post : ↑i5 = i.val + ↑j1_7) (i6 : U16) (i6_post : i6 = UScalar.cast UScalarTy.U16 coefficient2)
+  (pe_dst1 : Std.Array U16 256#usize) (pe_dst1_post : pe_dst1 = pe_dst1_7.set i5 i6) (j1 : Usize)
+  (j1_post : ↑j1 = j1_7.val + 1) (k : ℕ) (hk : k < 256) :
+  ((((((((Vector.set! (to_poly f) ↑i
+                                    ↑↑(UScalar.cast UScalarTy.U16
+                                          (core.num.U32.wrapping_add (core.num.U32.wrapping_sub i1_1 i2_1) i4_1))).set!
+                                (↑i + 1)
+                                ↑↑(UScalar.cast UScalarTy.U16
+                                      (core.num.U32.wrapping_add (core.num.U32.wrapping_sub i1_2 i2_2) i4_2))).set!
+                            (↑i + 2)
+                            ↑↑(UScalar.cast UScalarTy.U16
+                                  (core.num.U32.wrapping_add (core.num.U32.wrapping_sub i1_3 i2_3) i4_3))).set!
+                        (↑i + 3)
+                        ↑↑(UScalar.cast UScalarTy.U16
+                              (core.num.U32.wrapping_add (core.num.U32.wrapping_sub i1_4 i2_4) i4_4))).set!
+                    (↑i + 4)
+                    ↑↑(UScalar.cast UScalarTy.U16
+                          (core.num.U32.wrapping_add (core.num.U32.wrapping_sub i1_5 i2_5) i4_5))).set!
+                (↑i + 5)
+                ↑↑(UScalar.cast UScalarTy.U16
+                      (core.num.U32.wrapping_add (core.num.U32.wrapping_sub i1_6 i2_6) i4_6))).set!
+            (↑i + 6)
+            ↑↑(UScalar.cast UScalarTy.U16 (core.num.U32.wrapping_add (core.num.U32.wrapping_sub i1_7 i2_7) i4_7))).set!
+        (↑i + 7) ↑↑(UScalar.cast UScalarTy.U16 (core.num.U32.wrapping_add (core.num.U32.wrapping_sub i1 i2) i4)))[k] =
+    ((((((((Vector.set! (to_poly f) ↑i
+                                    ↑((4294967296 - (↑sample_bits &&& 15) >>> 2 + (↑sample_bits &&& 15 &&& 3) +
+                                          (3329 &&&
+                                            ((4294967296 - (↑sample_bits &&& 15) >>> 2 + (↑sample_bits &&& 15 &&& 3)) %
+                                                4294967296) >>>
+                                              16)) %
+                                        4294967296)).set!
+                                (↑i + 1)
+                                ↑((4294967296 - (↑sample_bits >>> 4 &&& 15) >>> 2 + (↑sample_bits >>> 4 &&& 15 &&& 3) +
+                                      (3329 &&&
+                                        ((4294967296 - (↑sample_bits >>> 4 &&& 15) >>> 2 +
+                                              (↑sample_bits >>> 4 &&& 15 &&& 3)) %
+                                            4294967296) >>>
+                                          16)) %
+                                    4294967296)).set!
+                            (↑i + 2)
+                            ↑((4294967296 - (↑sample_bits >>> 8 &&& 15) >>> 2 + (↑sample_bits >>> 8 &&& 15 &&& 3) +
+                                  (3329 &&&
+                                    ((4294967296 - (↑sample_bits >>> 8 &&& 15) >>> 2 +
+                                          (↑sample_bits >>> 8 &&& 15 &&& 3)) %
+                                        4294967296) >>>
+                                      16)) %
+                                4294967296)).set!
+                        (↑i + 3)
+                        ↑((4294967296 - (↑sample_bits >>> 12 &&& 15) >>> 2 + (↑sample_bits >>> 12 &&& 15 &&& 3) +
+                              (3329 &&&
+                                ((4294967296 - (↑sample_bits >>> 12 &&& 15) >>> 2 +
+                                      (↑sample_bits >>> 12 &&& 15 &&& 3)) %
+                                    4294967296) >>>
+                                  16)) %
+                            4294967296)).set!
+                    (↑i + 4)
+                    ↑((4294967296 - (↑sample_bits >>> 16 &&& 15) >>> 2 + (↑sample_bits >>> 16 &&& 15 &&& 3) +
+                          (3329 &&&
+                            ((4294967296 - (↑sample_bits >>> 16 &&& 15) >>> 2 + (↑sample_bits >>> 16 &&& 15 &&& 3)) %
+                                4294967296) >>>
+                              16)) %
+                        4294967296)).set!
+                (↑i + 5)
+                ↑((4294967296 - (↑sample_bits >>> 20 &&& 15) >>> 2 + (↑sample_bits >>> 20 &&& 15 &&& 3) +
+                      (3329 &&&
+                        ((4294967296 - (↑sample_bits >>> 20 &&& 15) >>> 2 + (↑sample_bits >>> 20 &&& 15 &&& 3)) %
+                            4294967296) >>>
+                          16)) %
+                    4294967296)).set!
+            (↑i + 6)
+            ↑((4294967296 - (↑sample_bits >>> 24 &&& 15) >>> 2 + (↑sample_bits >>> 24 &&& 15 &&& 3) +
+                  (3329 &&&
+                    ((4294967296 - (↑sample_bits >>> 24 &&& 15) >>> 2 + (↑sample_bits >>> 24 &&& 15 &&& 3)) %
+                        4294967296) >>>
+                      16)) %
+                4294967296)).set!
+        (↑i + 7)
+        ↑((4294967296 - (↑sample_bits >>> 28 &&& 15) >>> 2 + (↑sample_bits >>> 28 &&& 15 &&& 3) +
+              (3329 &&&
+                ((4294967296 - (↑sample_bits >>> 28 &&& 15) >>> 2 + (↑sample_bits >>> 28 &&& 15 &&& 3)) %
+                    4294967296) >>>
+                  16)) %
+            4294967296))[k] := sorry
+
+/-
+@[progress]
+def ntt.poly_element_sample_cbd_from_bytes_eta2_inner_loop_loop.spec (f : Array U16 256#usize)
+  (i : Usize) (sample_bits : U32) (hi1 : i.val < 256) (hi2 : 8 ∣ i.val) (j : Usize)
+  (hf : ∀ k < j.val, f[k]! = (Target2.samplePolyCBD.eta2_loop.inner_loop (to_poly f) i sample_bits).1[k]!)
+  :
+  ∃ f' sample_bits',
+  poly_element_sample_cbd_from_bytes_eta2_inner_loop_loop f i sample_bits j = ok (f', sample_bits') ∧
+  ∀ k < j.val, f'[k]! = (Target2.samplePolyCBD.eta2_loop.inner_loop (to_poly f) i sample_bits).1[k]! ∧
+  to_poly f' = (Target2.samplePolyCBD.eta2_loop.inner_loop (to_poly f) i sample_bits).1 ∧
+  sample_bits'.bv = (Target2.samplePolyCBD.eta2_loop.inner_loop (to_poly f) i sample_bits).2 := by
+-/
 
 -- This proof contains a lot of repeated code because `Target2.samplePolyCBD.eta2_loop.inner_loop` manually
 -- unfolds the loop body of `poly_element_sample_cbd_from_bytes_eta2_inner_loop` 8 times.
@@ -43,8 +243,16 @@ def ntt.poly_element_sample_cbd_from_bytes_eta2_inner_loop.spec (f : Array U16 2
   simp only [UScalar.lt_equiv, UScalar.ofNat_val_eq, Nat.ofNat_pos, ↓reduceIte, Q.eq, Spec.Q,
     BitVec.natCast_eq_ofNat, Bvify.UScalar.BitVec_ofNat_setWidth, UScalarTy.U32_numBits_eq,
     Bvify.U32.UScalar_bv, BitVec.setWidth_eq]
-  progress*
-  . simp only [U32.wrapping_add_val_eq, U32.wrapping_sub_val_eq, UScalar.val_and,
+  let* ⟨ coefficient, coefficient_post_1, coefficient_post_2 ⟩ ← UScalar.and_spec
+  let* ⟨ sample_bits1, sample_bits1_post_1, sample_bits1_post_2 ⟩ ← U32.ShiftRight_IScalar_spec
+  let* ⟨ i1, i1_post_1, i1_post_2 ⟩ ← UScalar.and_spec
+  let* ⟨ i2, i2_post_1, i2_post_2 ⟩ ← U32.ShiftRight_IScalar_spec
+  let* ⟨ coefficient1, coefficient1_post ⟩ ← core.num.U32.wrapping_sub.progress_spec
+  let* ⟨ i3, i3_post_1, i3_post_2 ⟩ ← U32.ShiftRight_IScalar_spec
+  let* ⟨ i4, i4_post_1, i4_post_2 ⟩ ← UScalar.and_spec
+  let* ⟨ coefficient2, coefficient2_post ⟩ ← core.num.U32.wrapping_add.progress_spec
+  let* ⟨ ⟩ ← massert_spec
+  · simp only [U32.wrapping_add_val_eq, U32.wrapping_sub_val_eq, UScalar.val_and,
       UScalar.ofNat_val_eq, UScalar.size_UScalarTyU32, Nat.mod_add_mod, coefficient2_post,
       coefficient1_post, i1_post_1, coefficient_post_1, i2_post_1, i4_post_1, i3_post_1]
     olet hsample_bits' : sample_bits' := sample_bits.val &&& 15
@@ -54,8 +262,166 @@ def ntt.poly_element_sample_cbd_from_bytes_eta2_inner_loop.spec (f : Array U16 2
       exact Nat.and_le_right
     revert sample_bits'
     brute
-  -- **TODO** Figure out how to proceed in a more modular way so that the proof doesn't slow down so much
-  sorry
+  let* ⟨ i5, i5_post ⟩ ← Usize.add_spec
+  let* ⟨ i6, i6_post ⟩ ← UScalar.cast.progress_spec
+  let* ⟨ pe_dst1, pe_dst1_post ⟩ ← Array.update_spec
+  let* ⟨ j1, j1_post ⟩ ← Usize.add_spec
+  unfold poly_element_sample_cbd_from_bytes_eta2_inner_loop_loop
+  simp only [UScalar.lt_equiv, j1_post, UScalar.ofNat_val_eq, Nat.one_lt_ofNat, ↓reduceIte, Q.eq]
+  let* ⟨ coefficient, coefficient_post_1, coefficient_post_2 ⟩ ← UScalar.and_spec
+  let* ⟨ sample_bits1, sample_bits1_post_1, sample_bits1_post_2 ⟩ ← U32.ShiftRight_IScalar_spec
+  let* ⟨ i1, i1_post_1, i1_post_2 ⟩ ← UScalar.and_spec
+  let* ⟨ i2, i2_post_1, i2_post_2 ⟩ ← U32.ShiftRight_IScalar_spec
+  let* ⟨ coefficient1, coefficient1_post ⟩ ← core.num.U32.wrapping_sub.progress_spec
+  let* ⟨ i3, i3_post_1, i3_post_2 ⟩ ← U32.ShiftRight_IScalar_spec
+  let* ⟨ i4, i4_post_1, i4_post_2 ⟩ ← UScalar.and_spec
+  let* ⟨ coefficient2, coefficient2_post ⟩ ← core.num.U32.wrapping_add.progress_spec
+  let* ⟨ ⟩ ← massert_spec
+  · sorry
+  let* ⟨ i5, i5_post ⟩ ← Usize.add_spec
+  let* ⟨ i6, i6_post ⟩ ← UScalar.cast.progress_spec
+  let* ⟨ pe_dst1, pe_dst1_post ⟩ ← Array.update_spec
+  let* ⟨ j1, j1_post ⟩ ← Usize.add_spec
+  unfold poly_element_sample_cbd_from_bytes_eta2_inner_loop_loop
+  split
+  . let* ⟨ coefficient, coefficient_post_1, coefficient_post_2 ⟩ ← UScalar.and_spec
+    let* ⟨ sample_bits1, sample_bits1_post_1, sample_bits1_post_2 ⟩ ← U32.ShiftRight_IScalar_spec
+    let* ⟨ i1, i1_post_1, i1_post_2 ⟩ ← UScalar.and_spec
+    let* ⟨ i2, i2_post_1, i2_post_2 ⟩ ← U32.ShiftRight_IScalar_spec
+    let* ⟨ coefficient1, coefficient1_post ⟩ ← core.num.U32.wrapping_sub.progress_spec
+    let* ⟨ i3, i3_post_1, i3_post_2 ⟩ ← U32.ShiftRight_IScalar_spec
+    let* ⟨ i4, i4_post_1, i4_post_2 ⟩ ← UScalar.and_spec
+    let* ⟨ coefficient2, coefficient2_post ⟩ ← core.num.U32.wrapping_add.progress_spec
+    let* ⟨ ⟩ ← massert_spec
+    · sorry
+    let* ⟨ i5, i5_post ⟩ ← Usize.add_spec
+    let* ⟨ i6, i6_post ⟩ ← UScalar.cast.progress_spec
+    let* ⟨ pe_dst1, pe_dst1_post ⟩ ← Array.update_spec
+    let* ⟨ j1, j1_post ⟩ ← Usize.add_spec
+    unfold poly_element_sample_cbd_from_bytes_eta2_inner_loop_loop
+    split
+    . let* ⟨ coefficient, coefficient_post_1, coefficient_post_2 ⟩ ← UScalar.and_spec
+      let* ⟨ sample_bits1, sample_bits1_post_1, sample_bits1_post_2 ⟩ ← U32.ShiftRight_IScalar_spec
+      let* ⟨ i1, i1_post_1, i1_post_2 ⟩ ← UScalar.and_spec
+      let* ⟨ i2, i2_post_1, i2_post_2 ⟩ ← U32.ShiftRight_IScalar_spec
+      let* ⟨ coefficient1, coefficient1_post ⟩ ← core.num.U32.wrapping_sub.progress_spec
+      let* ⟨ i3, i3_post_1, i3_post_2 ⟩ ← U32.ShiftRight_IScalar_spec
+      let* ⟨ i4, i4_post_1, i4_post_2 ⟩ ← UScalar.and_spec
+      let* ⟨ coefficient2, coefficient2_post ⟩ ← core.num.U32.wrapping_add.progress_spec
+      let* ⟨ ⟩ ← massert_spec
+      · sorry
+      let* ⟨ i5, i5_post ⟩ ← Usize.add_spec
+      let* ⟨ i6, i6_post ⟩ ← UScalar.cast.progress_spec
+      let* ⟨ pe_dst1, pe_dst1_post ⟩ ← Array.update_spec
+      let* ⟨ j1, j1_post ⟩ ← Usize.add_spec
+      unfold poly_element_sample_cbd_from_bytes_eta2_inner_loop_loop
+      split
+      . let* ⟨ coefficient, coefficient_post_1, coefficient_post_2 ⟩ ← UScalar.and_spec
+        let* ⟨ sample_bits1, sample_bits1_post_1, sample_bits1_post_2 ⟩ ← U32.ShiftRight_IScalar_spec
+        let* ⟨ i1, i1_post_1, i1_post_2 ⟩ ← UScalar.and_spec
+        let* ⟨ i2, i2_post_1, i2_post_2 ⟩ ← U32.ShiftRight_IScalar_spec
+        let* ⟨ coefficient1, coefficient1_post ⟩ ← core.num.U32.wrapping_sub.progress_spec
+        let* ⟨ i3, i3_post_1, i3_post_2 ⟩ ← U32.ShiftRight_IScalar_spec
+        let* ⟨ i4, i4_post_1, i4_post_2 ⟩ ← UScalar.and_spec
+        let* ⟨ coefficient2, coefficient2_post ⟩ ← core.num.U32.wrapping_add.progress_spec
+        let* ⟨ ⟩ ← massert_spec
+        · sorry
+        let* ⟨ i5, i5_post ⟩ ← Usize.add_spec
+        let* ⟨ i6, i6_post ⟩ ← UScalar.cast.progress_spec
+        let* ⟨ pe_dst1, pe_dst1_post ⟩ ← Array.update_spec
+        let* ⟨ j1, j1_post ⟩ ← Usize.add_spec
+        unfold poly_element_sample_cbd_from_bytes_eta2_inner_loop_loop
+        split
+        . let* ⟨ coefficient, coefficient_post_1, coefficient_post_2 ⟩ ← UScalar.and_spec
+          let* ⟨ sample_bits1, sample_bits1_post_1, sample_bits1_post_2 ⟩ ← U32.ShiftRight_IScalar_spec
+          let* ⟨ i1, i1_post_1, i1_post_2 ⟩ ← UScalar.and_spec
+          let* ⟨ i2, i2_post_1, i2_post_2 ⟩ ← U32.ShiftRight_IScalar_spec
+          let* ⟨ coefficient1, coefficient1_post ⟩ ← core.num.U32.wrapping_sub.progress_spec
+          let* ⟨ i3, i3_post_1, i3_post_2 ⟩ ← U32.ShiftRight_IScalar_spec
+          let* ⟨ i4, i4_post_1, i4_post_2 ⟩ ← UScalar.and_spec
+          let* ⟨ coefficient2, coefficient2_post ⟩ ← core.num.U32.wrapping_add.progress_spec
+          let* ⟨ ⟩ ← massert_spec
+          · sorry
+          let* ⟨ i5, i5_post ⟩ ← Usize.add_spec
+          let* ⟨ i6, i6_post ⟩ ← UScalar.cast.progress_spec
+          let* ⟨ pe_dst1, pe_dst1_post ⟩ ← Array.update_spec
+          let* ⟨ j1, j1_post ⟩ ← Usize.add_spec
+          unfold poly_element_sample_cbd_from_bytes_eta2_inner_loop_loop
+          split
+          . let* ⟨ coefficient, coefficient_post_1, coefficient_post_2 ⟩ ← UScalar.and_spec
+            let* ⟨ sample_bits1, sample_bits1_post_1, sample_bits1_post_2 ⟩ ← U32.ShiftRight_IScalar_spec
+            let* ⟨ i1, i1_post_1, i1_post_2 ⟩ ← UScalar.and_spec
+            let* ⟨ i2, i2_post_1, i2_post_2 ⟩ ← U32.ShiftRight_IScalar_spec
+            let* ⟨ coefficient1, coefficient1_post ⟩ ← core.num.U32.wrapping_sub.progress_spec
+            let* ⟨ i3, i3_post_1, i3_post_2 ⟩ ← U32.ShiftRight_IScalar_spec
+            let* ⟨ i4, i4_post_1, i4_post_2 ⟩ ← UScalar.and_spec
+            let* ⟨ coefficient2, coefficient2_post ⟩ ← core.num.U32.wrapping_add.progress_spec
+            let* ⟨ ⟩ ← massert_spec
+            · sorry
+            let* ⟨ i5, i5_post ⟩ ← Usize.add_spec
+            let* ⟨ i6, i6_post ⟩ ← UScalar.cast.progress_spec
+            let* ⟨ pe_dst1, pe_dst1_post ⟩ ← Array.update_spec
+            let* ⟨ j1, j1_post ⟩ ← Usize.add_spec
+            unfold poly_element_sample_cbd_from_bytes_eta2_inner_loop_loop
+            split
+            . let* ⟨ coefficient, coefficient_post_1, coefficient_post_2 ⟩ ← UScalar.and_spec
+              let* ⟨ sample_bits1, sample_bits1_post_1, sample_bits1_post_2 ⟩ ← U32.ShiftRight_IScalar_spec
+              let* ⟨ i1, i1_post_1, i1_post_2 ⟩ ← UScalar.and_spec
+              let* ⟨ i2, i2_post_1, i2_post_2 ⟩ ← U32.ShiftRight_IScalar_spec
+              let* ⟨ coefficient1, coefficient1_post ⟩ ← core.num.U32.wrapping_sub.progress_spec
+              let* ⟨ i3, i3_post_1, i3_post_2 ⟩ ← U32.ShiftRight_IScalar_spec
+              let* ⟨ i4, i4_post_1, i4_post_2 ⟩ ← UScalar.and_spec
+              let* ⟨ coefficient2, coefficient2_post ⟩ ← core.num.U32.wrapping_add.progress_spec
+              let* ⟨ ⟩ ← massert_spec
+              · sorry
+              let* ⟨ i5, i5_post ⟩ ← Usize.add_spec
+              let* ⟨ i6, i6_post ⟩ ← UScalar.cast.progress_spec
+              let* ⟨ pe_dst1, pe_dst1_post ⟩ ← Array.update_spec
+              let* ⟨ j1, j1_post ⟩ ← Usize.add_spec
+              unfold poly_element_sample_cbd_from_bytes_eta2_inner_loop_loop
+              simp only [UScalar.lt_equiv, Nat.reduceAdd, UScalar.ofNat_val_eq, lt_self_iff_false,
+                ↓reduceIte, ok.injEq, Prod.mk.injEq, and_assoc, exists_and_left, exists_eq_left',
+                BitVec.reduceShiftRightShiftRight, to_poly_set, Spec.Q, add_zero, *]
+              unfold Target2.samplePolyCBD.eta2_loop.inner_loop
+                Target2.samplePolyCBD.eta2_loop.inner_loop.next_coefficient
+              simp only [BitVec.ofNat_eq_ofNat, Q.eq, UScalar.ofNat_val_eq, Nat.cast_ofNat,
+                BitVec.toNat_add, BitVec.toNat_sub, Nat.reducePow, BitVec.toNat_ushiftRight,
+                BitVec.toNat_and, UScalar.bv_toNat, BitVec.toNat_ofNat, Nat.reduceMod,
+                Nat.mod_add_mod, BitVec.reduceShiftRightShiftRight, and_true]
+              ext k hk
+              -- `apply ntt.poly_element_sample_cbd_from_bytes_eta2_inner_loop.spec.aux` struggles
+              -- to instantiate all of the arguments
+              sorry
+            . simp only [progress_simps]
+              scalar_tac
+          . simp only [progress_simps]
+            scalar_tac
+        . simp only [progress_simps]
+          scalar_tac
+      . simp only [progress_simps]
+        scalar_tac
+    . simp only [progress_simps]
+      scalar_tac
+  . simp only [progress_simps]
+    scalar_tac
+
+  /-
+  let f' : Std.Array U16 256#usize := sorry
+  have hsample_bits' : ∃ sample_bits' : U32, sample_bits'.bv = sample_bits.bv >>> 32 := by
+    apply Exists.intro $ U32.ofNat (sample_bits.val >>> 32) (by scalar_tac)
+    simp
+  rcases hsample_bits' with ⟨sample_bits', hsample_bits'⟩
+  apply Exists.intro f'
+  apply Exists.intro sample_bits'
+  split_conjs
+  . sorry
+  . sorry
+  . simp only [hsample_bits', Target2.samplePolyCBD.eta2_loop.inner_loop, Spec.Q,
+      Target2.samplePolyCBD.eta2_loop.inner_loop.next_coefficient, BitVec.ofNat_eq_ofNat, Q.eq,
+      UScalar.ofNat_val_eq, Nat.cast_ofNat, BitVec.toNat_add, BitVec.toNat_sub, Nat.reducePow,
+      BitVec.toNat_ushiftRight, BitVec.toNat_and, UScalar.bv_toNat, BitVec.toNat_ofNat, Nat.reduceMod,
+      Nat.mod_add_mod, BitVec.reduceShiftRightShiftRight]
+  -/
   /-
   unfold poly_element_sample_cbd_from_bytes_eta2_inner_loop_loop
   simp only [UScalar.lt_equiv, j1_post, UScalar.ofNat_val_eq, Nat.one_lt_ofNat, ↓reduceIte, Q.eq]
